add new consistent state def

proofs/zero_coupon_bond.v
@@ -1,4 +1,4 @@
-Load metaproperties.
+Load findel.
 
 (* Zero coupon bond *)
 Definition zcb_desc
@@ -9,11 +9,317 @@ Definition zcb_desc
      (At (NOW + PERIOD) (Scale 11 (One USD)))
   ).
 
+Definition executed
+           (ctr : FinContract)
+           (s s' : State)
+           (at_ : Time) :=
+    step s s' /\
+    In ctr (m_contracts s) /\
+    In (Executed ctr) (m_events s') /\
+    at_ = m_global_time s.
+
+Definition deleted
+           (ctr : FinContract)
+           (s s' : State)
+           (at_ : Time) :=
+    step s s' /\
+    In ctr (m_contracts s) /\
+    In (Deleted ctr) (m_events s') /\
+    at_ = m_global_time s.
+
+Definition joins
+           (O : Address)
+           (ctr : FinContract)
+           (s1 s2 : State)
+           (at_ : Time) :=
+   exists s s', (s1 ~~> s) /\ (s' ~~> s2) /\ (executed ctr s s' at_ \/ deleted ctr s s' at_).
+
+Ltac destruct_executed H :=
+  let S := fresh "St" in
+  let M := fresh "M" in
+  let Ev := fresh "Ev" in
+  let T := fresh "T" in
+  destruct H as [S [M [Ev T]]].
+
+Ltac destruct_deleted := destruct_executed.
+
+Ltac destruct_join H :=
+  let s := fresh "s" in
+  let s' := fresh "s'" in
+  let Ss1 := fresh "Ss" in
+  let Ss2 := fresh "Ss" in
+  let E := fresh "E" in
+  let D := fresh "D" in
+  destruct H as [s [s' [Ss1 [Ss2 [E | D]]]]]; try destruct_executed E; try destruct_deleted D.
+
+Definition consistent' (s : State) :=
+    (forall ctr, In ctr (m_contracts s) -> ~ In (Executed ctr) (m_events s)) /\
+    (forall ctr, In ctr (m_contracts s) -> ~ In (Deleted ctr) (m_events s)) /\
+    (forall ctr, In (Executed ctr) (m_events s) -> ~ In (Deleted ctr) (m_events s)) /\
+    (forall ctr, In (Deleted ctr) (m_events s) -> ~ In (Executed ctr) (m_events s)) /\
+    next_id_is_fresh s.
+Print State.
+
+Lemma new_contract_is_fresh :
+  forall ctr s,
+    ctr_id ctr = m_fresh_id s ->
+    next_id_is_fresh s ->
+    ~ In ctr (m_contracts s).
+Proof.
+  intros ctr s H [H1 [H2 [H3 H4]]].
+  unfold not. intros C.
+  apply H1 in C.
+  contradiction.
+Qed.
+
+Lemma new_contracts_are_not_executed :
+  forall ctr s,
+    ctr_id ctr = m_fresh_id s ->
+    next_id_is_fresh s ->
+    ~ In (Executed ctr) (m_events s).
+Proof.
+  intros ctr s H [H1 [H2 [H3 H4]]].
+  unfold not. intros C.
+  apply H2 in C.
+  contradiction.
+Qed.
+    
+Lemma new_contracts_are_not_deleted :
+  forall ctr s,
+    ctr_id ctr = m_fresh_id s ->
+    next_id_is_fresh s ->
+    ~ In (Deleted ctr) (m_events s).
+Proof.
+  intros ctr s H [H1 [H2 [H3 H4]]].
+  unfold not. intros C.
+  apply H3 in C.
+  contradiction.
+Qed.
+
+Ltac unfold_append :=
+  unfold not; intros CL;
+  unfold append_new_ctr_to_state in *; simpl in *;
+  destruct CL as [CL | CL].
+Ltac resolve_append :=
+  unfold_append; try inversion CL.  
+
+Lemma rm_in:
+  forall cs c, In c (rm c cs) -> False.
+Proof.
+  induction cs; intros; simpl in *; try contradiction.
+  case_eq (FinContract_eq_dec c a); intros H0 H'; rewrite H' in H.
+  + eapply IHcs. eauto.
+  + simpl in H. destruct H as [H | H]. subst. contradiction.
+    eapply IHcs. eauto.
+Qed.
+
+Lemma incl_rm : forall S x y, x <> y -> In x (rm y S) -> In x S.
+Proof.
+  induction S.
+  - simpl. intros. trivial.
+  - intros.
+    simpl in H0.
+    case_eq (FinContract_eq_dec y a); intros He H'; rewrite H' in H0. subst.
+    + simpl. right. eapply IHS; eauto.
+    + simpl in H0. destruct H0 as [H0 | H0]; subst.
+      * simpl. left. reflexivity.
+      * simpl. right. eapply IHS; eauto.
+Qed.
+
+Lemma new_contracts_are_fresh :
+  forall ctr s owner bal' ctrs' next' ledger',
+    consistent' s ->
+    next_id_is_fresh s ->
+    exec_ctr_in_state_with_owner ctr s owner = Some (result bal' ctrs' next' ledger') ->
+    ~ In ctr ctrs'.
+Proof.
+  intros ctr.
+  destruct ctr.
+  induction ctr_primitive0; intros s owner bal' ctrs' next' ledger' C F E; unfold exec_ctr_in_state_with_owner in E; simpl in E.
+  - try inversion E; clear E. subst. auto.
+  - try inversion E; clear E. subst. auto.
+  -     
+    
+  unfold not. intros CTR.
+  destruct ctr.
+  unfold exec_ctr_in_state_with_owner in E.
+  induction ctr_primitive0; simpl in E.
+  - try inversion E; clear E; try subst ctrs'; trivial.
+  - try inversion E; clear E; try subst ctrs'; trivial.
+  - simpl in *.apply IHctr_primitive0.
+  - simpl in *. apply IHctr_primitive0 in CTR. ; eauto.
+  - 
+  
+
+Lemma consistent_step_1 : forall  (s s' : State),
+  step s s' ->
+  consistent' s ->
+  (forall ctr, In ctr (m_contracts s') -> ~ In (Executed ctr) (m_events s')).
+Proof.
+  intros s s' H (C1 & _).
+  destruct H; subst s'.
+  - unfold not. intros. simpl in H4, H5.
+    destruct H5 as [H5 | H5]; try inversion H5.
+    + destruct H4 as [H4 | H4].
+      * subst ctr.
+        apply new_contracts_are_not_executed with (ctr := new_contract) in H5; try contradiction; subst; trivial.
+      * apply C1 in H4. contradiction.
+  - unfold not. intros. simpl in *.
+    rewrite in_app_iff in H6. 
+    destruct H6 as [H6 | H6].
+    case_eq (FinContract_eq_dec ctr ctr0); intros.
+    + subst ctr0.
+      destruct H7 as [H7 | H7]; try eapply rm_in; eauto.
+    + destruct H7 as [H7 | H7]. 
+      * inversion H7. try contradiction.
+      * apply incl_rm in H6; auto. apply C1 in H6. contradiction.
+    + destruct H7 as [H7 | H7].
+      * inversion H7. subst.
+
+
+
+        
+        apply 
+      
+      * inversion H7. clear H7. subst ctr0.
+        eapply rm_in; eauto.
+      * unfold not in C1. apply C1 with (ctr := ctr0).
+        case_eq (FinContract_eq_dec ctr ctr0); intros.
+
+          
+
+          
+
+      try inversion H6.
+    + destruct H4 as [H4 | H4].
+      * subst ctr.
+        apply new_contracts_are_not_executed with (ctr := new_contract) in H5; try contradiction; subst; trivial.
+      * apply C1 in H4. contradiction.
+  -
+    
+    intros FG.
+  - simpl in H', FG.
+    destruct H' as [H' | H'].
+    + subst ctr'.
+      apply new_contracts_are_not_executed with (ctr := new_contract) in H3.
+      contradiction. subst. trivial.
+    + resolve_append.
+      
+    unfold_append.
+    
+
+  apply C1; trivial.
+Qed.    
+
+Lemma consistent_step_2 : forall  (s s' : State),
+  step s s' ->
+  consistent' s ->
+  (forall ctr, In ctr (m_contracts s) -> ~ In (Deleted ctr) (m_events s)).
+Proof.
+  intros s s' H (_ & C2 & _).
+  destruct H; subst s'; intros ctr' H'; apply C2; trivial.
+Qed.
+
+Lemma consistent_step_3 : forall  (s s' : State),
+  step s s' ->
+  consistent' s ->
+  (forall ctr, In (Executed ctr) (m_events s) -> ~ In (Deleted ctr) (m_events s)).
+Proof.
+  intros s s' H (C1 & C2 & C3 & C4 & F).
+  destruct H; subst s'; intros ctr' H'; apply C3; trivial.
+Qed.
+
+Lemma consistent_step_4 : forall  (s s' : State),
+  step s s' ->
+  consistent' s ->
+  (forall ctr, In (Deleted ctr) (m_events s) -> ~ In (Executed ctr) (m_events s)).
+Proof.
+  intros s s' H (C1 & C2 & C3 & C4 & F).
+  destruct H; subst s'; intros ctr' H'; apply C4; trivial.
+Qed.
+
+Lemma consistent_step_5 : forall  (s s' : State),
+  step s s' ->
+  consistent' s ->
+  next_id_is_fresh s'.
+  
+
+    simpl in H'. destruct H' as [H' | H'].
+      * unfold_append. subst ctr. inversion CL.
+        apply new_contracts_are_not_executed with (ctr := ctr) in F.
+        contradiction. subst; auto.
+      * resolve_append. apply C1 in H'. contradiction.
+    + intros ctr H'. simpl in H'. destruct H' as [H' | H'].
+      * unfold_append. subst ctr. inversion CL.
+        apply new_contracts_are_not_deleted with (ctr := ctr) in F.
+        contradiction. subst; auto.
+      * resolve_append. apply C2 in H'. contradiction.
+    + intros ctr H'. simpl in H'. destruct H' as [H' | H'].
+      * inversion H'.
+      * unfold_append. inversion CL.
+        apply C3 in H'. contradiction.
+    + intros ctr H'. simpl in H'. destruct H' as [H' | H'].
+      * inversion H'.
+      * unfold_append. inversion CL.
+        apply C4 in H'. contradiction.
+  
+  
+Lemma consistent_step : forall  (s s' : State),
+  step s s' ->
+  consistent' s ->
+  consistent' s'.
+Proof.
+  intros s s' H (C1 & C2 & C3 & C4 & F).
+  destruct H; subst s'.
+  - repeat split.
+    + intros ctr H'. simpl in H'. destruct H' as [H' | H'].
+      * unfold_append. subst ctr. inversion CL.
+        apply new_contracts_are_not_executed with (ctr := ctr) in F.
+        contradiction. subst; auto.
+      * resolve_append. apply C1 in H'. contradiction.
+    + intros ctr H'. simpl in H'. destruct H' as [H' | H'].
+      * unfold_append. subst ctr. inversion CL.
+        apply new_contracts_are_not_deleted with (ctr := ctr) in F.
+        contradiction. subst; auto.
+      * resolve_append. apply C2 in H'. contradiction.
+    + intros ctr H'. simpl in H'. destruct H' as [H' | H'].
+      * inversion H'.
+      * unfold_append. inversion CL.
+        apply C3 in H'. contradiction.
+    + intros ctr H'. simpl in H'. destruct H' as [H' | H'].
+      * inversion H'.
+      * unfold_append. inversion CL.
+        apply C4 in H'. contradiction.
+    + 
+        unfold_append. subst ctr. inversion CL.
+        apply new_contracts_are_not_deleted with (ctr := ctr) in F.
+        contradiction. subst; auto.
+      * resolve_append. apply C2 in H'. contradiction.
+
+    +    
+Admitted.
+
+Lemma consistent_steps : forall  (s s' : State),
+  steps s s' ->
+  consistent' s ->
+  consistent' s'.
+Admitted.
+
+Ltac insert_consistent' s H :=
+  let H' := fresh "H" in
+  match goal with
+  | H : steps _ s |- _ => 
+    assert (H' : consistent' s);
+    try eapply consistent_steps; eauto
+  | H : step _ s |- _ =>
+    assert (H' : consistent' s);
+    try eapply consistent_step;eauto
+  end.
 
 (* The issuer's rights *)
 Proposition zcb_O_to_I:
   forall s1 s2 ctr_id dsc_id now period I O sc ctr,
-    consistent_state s1 ->
+    consistent' s1 ->
     ctr = finctr ctr_id dsc_id (zcb_desc now period) I O O sc ->
     joins O ctr s1 s2 now ->
     O <> 0 ->
@@ -25,7 +331,59 @@ Proposition zcb_O_to_I:
       tr_amount tr = sc * 10.
 Proof.
   intros.
-  destruct_join H1.
+  destruct_join H1;
+  insert_consistent' s Ss;
+  insert_consistent' s' St;
+  insert_consistent' s2 St.
+  - induction St; subst s'; simpl in Ev.
+    + destruct Ev as [Ev | Ev].
+      inversion Ev.
+      unfold consistent' in H1.
+      destruct H1 as (C & _ & _ & _ & _ & _).
+      apply C in M. contradiction.
+    + destruct Ev as [Ev | Ev].
+      * admit.
+      * destruct H1 as (C & _ & _ & _ & _ & _).
+        apply C in M. contradiction.
+    + destruct Ev as [Ev | Ev].
+      * admit.
+      * destruct H1 as (C & _ & _ & _ & _ & _).
+        apply C in M. contradiction.
+    + destruct Ev as [Ev | Ev].
+      * admit.
+      * destruct H1 as (C & _ & _ & _ & _ & _).
+        apply C in M. contradiction.
+    + destruct Ev as [Ev | Ev].
+      * admit.
+      * destruct H1 as (C & _ & _ & _ & _ & _).
+        apply C in M. contradiction.
+    + destruct H1 as (C & _ & _ & _ & _ & _).
+      apply C in M. contradiction.
+  - induction St; subst s'; simpl in Ev.
+    + destruct Ev as [Ev | Ev]. inversion Ev.
+      destruct H1 as (_ & C & _ & _ & _ & _).
+      apply C in M. contradiction.
+    + destruct Ev as [Ev | Ev].
+      * inversion Ev.
+      * destruct H1 as (_ & C & _ & _ & _ & _).
+        apply C in M. contradiction.
+    + destruct Ev as [Ev | Ev].
+      * inversion Ev.
+      * destruct H1 as (_ & C & _ & _ & _ & _).
+        apply C in M. contradiction.
+    + destruct Ev as [Ev | Ev].
+      * inversion Ev.
+      * destruct H1 as (_ & C & _ & _ & _ & _).
+        apply C in M. contradiction.
+    + destruct Ev as [Ev | Ev].
+      * inversion Ev. admit.
+      * destruct H1 as (_ & C & _ & _ & _ & _).
+        apply C in M. contradiction.
+    + destruct H1 as (_ & C & _ & _ & _ & _).
+      apply C in M. contradiction.
+Qed.
+        
+    
   - insert_consistent s Ss.
     induction St; subst s'.
     + inversion_event Ev. find_contradiction M.
